move some invs into common

glue/generic_falcon_lemmas.dfy
@@ -13,18 +13,6 @@ abstract module generic_falcon_lemmas {
 
     import FNTT = falcon_512_i.FNTT
     import INTT = falcon_512_i.INTT
-    import opened MQP = falcon_512_i.CMQP
-
-    const Q := falcon_512_i.Q;
-    const N := falcon_512_i.N; 
-    const OMEGA := falcon_512_i.CMQ.OMEGA;
-
-    const R := CMQ.R;
-    const PSI := CMQ.PSI;
-
-    type floop_view = FNTT.loop_view
-
-    type iloop_view = INTT.loop_view
 
     predicate {:opaque} buff_is_n_elems(a: seq<nat>)
         ensures buff_is_n_elems(a) ==> |a| == N.full;
@@ -41,28 +29,29 @@ abstract module generic_falcon_lemmas {
         a
     }
 
-    function block_size(d: pow2_t): pow2_t
-        requires CPV.block_size.requires(d)
-    {
-        CPV.block_size(d)
-    }
-
-    function build_floop_view(s: n_elems, d: pow2_t): floop_view
-        requires FNTT.build_loop_view.requires(s, d)
-    {
-        FNTT.build_loop_view(s, d)
-    }
-
-    function build_iloop_view(s: n_elems, d: pow2_t): iloop_view
-        requires INTT.build_loop_view.requires(s, d)
-    {
-        INTT.build_loop_view(s, d)
-    }
+// mq arith wraps
 
     function montmul(a: elem, b: elem): elem
     {
         MQP.montmul(a, b)
     }
+
+    function mqadd(a: elem, b: elem): elem
+    {
+        MQP.mqadd(a, b)
+    }
+
+    function mqsub(a: elem, b: elem): elem
+    {
+        MQP.mqsub(a, b)
+    }
+
+    function mqmul(a: elem, b: elem): elem
+    {
+        MQP.mqmul(a, b)
+    }
+
+// table wraps
 
     function rev_mixed_powers_mont_x_value(i: nat, d: pow2_t): (r: elem)
     {
@@ -89,5 +78,103 @@ abstract module generic_falcon_lemmas {
         MQP.inverse_ntt_scaling_table()
     }
 
+// fntt wraps
+    type floop_view = FNTT.loop_view
 
+    function block_size(d: pow2_t): pow2_t
+        requires CPV.block_size.requires(d)
+    {
+        CPV.block_size(d)
+    }
+
+    function build_floop_view(s: n_elems, d: pow2_t): floop_view
+        requires FNTT.build_loop_view.requires(s, d)
+    {
+        FNTT.build_loop_view(s, d)
+    }
+
+    function forward_lsize(view: FNTT.loop_view): (r: pow2_t)
+        requires view.loop_view_wf();
+        ensures r.full <= N.full
+    {
+        view.lsize()
+    }
+
+    predicate forward_ntt_eval_all(a: seq<nat>, coeffs: seq<nat>)
+    {
+        && buff_is_n_elems(a)
+        && buff_is_n_elems(coeffs)
+        && FNTT.ntt_eval_all(buff_as_n_elems(a), buff_as_n_elems(coeffs))
+    }
+
+    predicate forward_t_loop_inv(a: seq<nat>, d: pow2_t, coeffs: seq<nat>)
+        requires 0 <= d.exp <= N.exp;
+    {
+        && buff_is_n_elems(a)
+        && buff_is_n_elems(coeffs)
+        && FNTT.t_loop_inv(buff_as_n_elems(a), d, buff_as_n_elems(coeffs))
+    }
+
+    predicate forward_s_loop_inv(a: seq<nat>, d: pow2_t, j: nat, bi: nat, view: FNTT.loop_view)
+    {
+        && buff_is_n_elems(a)
+        && view.s_loop_inv(buff_as_n_elems(a), d, j, bi)
+    }
+
+    predicate forward_j_loop_inv(a: seq<nat>, d: pow2_t, j: nat, u: nat, view: FNTT.loop_view)
+    {
+        && buff_is_n_elems(a)
+        && u == j * (2 * d.full)
+        && view.j_loop_inv(buff_as_n_elems(a), d, j)
+    }
+
+    lemma forward_t_loop_inv_pre_lemma(coeffs: seq<nat>)
+        requires buff_is_n_elems(coeffs);
+        ensures N.exp <= N.exp; // ??
+        ensures forward_t_loop_inv(coeffs, N, coeffs);
+    {
+        FNTT.t_loop_inv_pre_lemma(buff_as_n_elems(coeffs));
+    }
+
+    lemma forward_t_loop_inv_post_lemma(a: seq<nat>, one: pow2_t, coeffs: seq<nat>)
+        requires one.exp == 0 <= N.exp;
+        requires forward_t_loop_inv(a, one, coeffs);
+        ensures forward_ntt_eval_all(a, coeffs);
+    {
+        FNTT.t_loop_inv_post_lemma(a, one, coeffs);
+    }
+
+// intt wraps
+    type iloop_view = INTT.loop_view
+
+    function build_iloop_view(s: n_elems, d: pow2_t): iloop_view
+        requires INTT.build_loop_view.requires(s, d)
+    {
+        INTT.build_loop_view(s, d)
+    }
+
+// polysub wraps
+    predicate poly_sub_loop_inv(diff: seq<nat>, f: seq<nat>, g: seq<nat>, i: nat)
+    {
+        reveal buff_is_n_elems();
+        && buff_is_n_elems(diff)
+        && buff_is_n_elems(f)
+        && buff_is_n_elems(g)
+        && 0 <= i <= N.full
+        && diff[i..] == f[i..]
+        && (forall j | 0 <= j < i :: diff[j] == MQP.mqsub(f[j], g[j]))
+    }
+
+    lemma poly_sub_loop_correct(f_new: seq<nat>, f_old: seq<nat>, f_orig:seq<nat>, g: seq<nat>, i: nat)
+        requires i < N.full;
+        requires poly_sub_loop_inv(f_old, f_orig, g, i)
+        requires f_new == f_old[i := MQP.mqsub(f_orig[i], g[i])];
+        ensures poly_sub_loop_inv(f_new, f_orig, g, i+1);
+    {
+        assert |f_new| == |f_old|;
+        forall j | 0 <= j < |f_new|
+            ensures j != i ==> f_new[j] == f_old[j];
+            ensures j == i ==> f_new[j] == MQP.mqsub(f_orig[j], g[j]);
+        {}
+    }
 }
