spec/crypto/falcon.s.dfy
@@ -4,22 +4,20 @@ include "mq_norm.s.dfy"
 abstract module falcon_s(MQ: ntt_param_s, MQP: mq_poly_s(MQ)) {
     import MQN = mq_norm_s(MQ)
 
-    type elem = MQ.elem
-    type n_elems = MQ.n_elems
-    type nelem = MQN.nelem
-
-    const Q := MQ.Q;
-    const N := MQ.N; 
-
     function bound(): nat
 
-    predicate falcon_verify(c0: seq<elem>, s2: seq<nelem>, h: seq<elem>)
-        requires |c0| == |s2| == |h| == N.full;
+    function poly_mod_product(a: seq<MQ.elem>, b: seq<MQ.elem>): (p: seq<MQ.elem>)
+    {
+        MQP.poly_mod(MQP.poly_mul(a, b), MQP.n_ideal())
+    }
+
+    predicate falcon_verify(c0: seq<MQ.elem>, s2: seq<MQN.nelem>, h: seq<MQ.elem>)
+        requires |c0| == |s2| == |h| == MQ.N.full;
     {
         var tt0 := MQN.denormalize_n_elems(s2);
-        var tt1 := MQP.poly_mod(MQP.poly_mul(tt0, h), MQP.n_ideal());
+        var tt1 := poly_mod_product(tt0, h);
         var tt2 := MQP.poly_sub(tt1, c0);
         var s1 := MQN.normalize_elems(tt2);
-        MQN.l2norm_squared(s1, s2, N.full) < bound()
+        MQN.l2norm_squared(s1, s2, MQ.N.full) < bound()
     }
 }
